Use stdpp set (2) (#30)
* generalize and collect extensions to the stdpp library

* use stdpp set almost everywhere

instead of list sets

src/locally_nameless.v
@@ -7,7 +7,7 @@ Require Import Coq.micromega.Lia.
 
 (*From Equations Require Import Equations.*)
 Require Export String.
-Require Export Coq.Lists.ListSet.
+(*Require Export Coq.Lists.ListSet.*)
 Require Export Ensembles_Ext.
 
 Require Export Coq.Program.Wf.
@@ -16,6 +16,82 @@ From stdpp Require Import pmap gmap mapset fin_sets.
 
 Require Import Lattice.
 Require Import Signature.
+
+(* Extensions to the stdpp library *)
+Section stdpp_ext.
+
+  Lemma pmap_to_list_lookup {A} (M : Pmap A) (i : positive) (x : A)
+  : (i,x) ∈ (map_to_list M) <-> lookup i M = Some x.
+  Proof.
+    intros. unfold map_to_list. unfold Pto_list. unfold lookup. unfold Plookup.
+    destruct M eqn:HM. simpl.
+    split; intros.
+    + apply Pelem_of_to_list in H. simpl in H.
+      destruct H.
+      * destruct H as [i' [Hi' Hsome]]. subst. apply Hsome.
+      * inversion H.
+    + apply Pelem_of_to_list.
+      left. simpl. exists i. firstorder.
+  Qed.
+
+  Lemma gmap_to_list_lookup `{Countable K} {A} (M : gmap K A) (k : K) (a : A): ((k,a) ∈ (gmap_to_list M)) <-> (M !! k = Some a).
+  Proof.
+    unfold elem_of.
+    unfold lookup.
+    destruct M as [PM PMwf] eqn: HM. simpl.
+    unfold gmap_wf in PMwf.
+    split; intros H'.
+    + apply pmap_to_list_lookup.
+      apply elem_of_list_omap in H'.
+      destruct H' as [[k' a'] [HxinPM H']].
+      apply fmap_Some_1 in H'.
+      destruct H' as [k'' [H1 H2]]. inversion H2. subst. clear H2.
+      assert (Hk': k' = encode k'').
+      { apply bool_decide_unpack in PMwf.
+        unfold map_Forall in PMwf.
+        apply pmap_to_list_lookup in HxinPM.
+        specialize (PMwf k' a' HxinPM).
+        apply (inj Some). rewrite <- PMwf.
+        apply fmap_Some_2. apply H1. }
+      subst. apply HxinPM.
+      
+    + apply pmap_to_list_lookup in H'.
+      apply elem_of_list_omap.
+      exists (encode k, a). firstorder.
+      rewrite -> decode_encode. simpl. reflexivity.
+  Qed.
+
+  Program Instance inj_unit_r : @Inj (K * ()) K (@eq (K * ())) (@eq K) (@fst K ()).
+  Next Obligation.
+    intros. destruct x,y. simpl in H. subst. destruct u. destruct u0. reflexivity.
+  Defined.
+
+  Lemma gset_to_list_elem_of `{Countable K} (S : gset K) (k : K) : k ∈ (mapset_elements S) <-> k ∈ S.
+  Proof.
+    unfold mapset_elements.
+    destruct S as [M].
+    unfold elem_of at 2.
+    unfold gset_elem_of. unfold mapset_elem_of. simpl.
+    rewrite <- gmap_to_list_lookup.
+    unfold map_to_list.
+    assert (Hk : k = fst (k, ())).
+    { reflexivity. }
+    rewrite -> Hk at 1.
+    split; intros H'.
+    + apply elem_of_list_fmap_2_inj in H'. apply H'.
+      apply inj_unit_r.
+    + apply elem_of_list_fmap_1. assumption.
+  Qed.
+
+  Lemma mapset_elements_to_set `{Countable K} (X : gset K) : list_to_set (mapset_elements X) = X.
+  Proof.
+    apply (iffRL (@mapset_eq K (gmap K) _ _ _ _ _ _ _ _ gmap_finmap _ _)).
+    intros x. 
+    pose proof (H' := @elem_of_list_to_set K (gset K) _ _ _ _ _ x (mapset_elements X)).
+    rewrite -> H'. apply gset_to_list_elem_of.
+  Qed.
+
+End stdpp_ext.
 
 (** ** Matching Logic Syntax *)
 Section ml_syntax_semantics.
@@ -146,14 +222,8 @@ end.
 (** The free names of a type are defined as follow.  Notice the
   [exists] and [mu] cases: they do not bind any name. *)
 
-
-(*Notation EVarSet := (mapset (@gmap evar evar_eqdec evar_countable)).*)
-
 Notation EVarSet := (@gset evar evar_eqdec evar_countable).
-
-Definition set_singleton {T : Type}
-  (eq : forall (x y : T), { x = y } + { x <> y })
-  := fun x : T => set_add eq x List.nil.
+Notation SVarSet := (@gset svar svar_eqdec svar_countable).
 
 Fixpoint free_evars (phi : Pattern)
   : EVarSet :=
@@ -171,16 +241,16 @@ match phi with
 end.
 
 Fixpoint free_svars (phi : Pattern)
-  : (ListSet.set svar) :=
+  : SVarSet :=
 match phi with
-| patt_free_evar x => List.nil
-| patt_free_svar X => set_singleton svar_eq X
-| patt_bound_evar x => List.nil
-| patt_bound_svar X => List.nil
-| patt_sym sigma => List.nil
-| patt_app phi1 phi2 => set_union svar_eq (free_svars phi1) (free_svars phi2)
-| patt_bott => List.nil
-| patt_imp phi1 phi2 => set_union svar_eq (free_svars phi1) (free_svars phi2)
+| patt_free_evar x => empty
+| patt_free_svar X => singleton X
+| patt_bound_evar x => empty
+| patt_bound_svar X => empty
+| patt_sym sigma => empty
+| patt_app phi1 phi2 => union (free_svars phi1) (free_svars phi2)
+| patt_bott => empty
+| patt_imp phi1 phi2 => union (free_svars phi1) (free_svars phi2)
 | patt_exists phi => free_svars phi
 | patt_mu phi => free_svars phi
 end.
@@ -191,6 +261,8 @@ end.
 
 Record Model := {
   Domain : Type;
+  (* TODO think about whether or not to make it an existential formula. Because that would affect the equality,
+     due to proof irrelevance. *)
   nonempty_witness : Domain;
   Domain_eq_dec : forall (a b : Domain), {a = b} + {a <> b};
   app_interp : Domain -> Domain -> Power Domain;
@@ -586,82 +658,25 @@ Proof.
   apply wfc_aux_body_ex_imp1. auto.
 Qed.
 
-Lemma pmap_to_list_lookup {A} (M : Pmap A) (i : positive) (x : A)
-  : (i,x) ∈ (map_to_list M) <-> lookup i M = Some x.
-Proof.
-  intros. unfold map_to_list. unfold Pto_list. unfold lookup. unfold Plookup.
-  destruct M eqn:HM. simpl.
-  split; intros.
-  + apply Pelem_of_to_list in H. simpl in H.
-    destruct H.
-    * destruct H as [i' [Hi' Hsome]]. subst. apply Hsome.
-    * inversion H.
-  + apply Pelem_of_to_list.
-    left. simpl. exists i. firstorder.
-Qed.
+Definition fresh_evar ϕ := evar_fresh (elements (free_evars ϕ)).
+Definition fresh_svar ϕ := svar_fresh (elements (free_svars ϕ)).
 
-Lemma gmap_to_list_lookup `{Countable K} {A} (M : gmap K A) (k : K) (a : A): ((k,a) ∈ (gmap_to_list M)) <-> (M !! k = Some a).
+Lemma set_evar_fresh_is_fresh ϕ : fresh_evar ϕ ∉ free_evars ϕ.
 Proof.
-  unfold elem_of.
-  unfold lookup.
-  destruct M as [PM PMwf] eqn: HM. simpl.
-  unfold gmap_wf in PMwf.
-  split; intros H'.
-  + apply pmap_to_list_lookup.
-    apply elem_of_list_omap in H'.
-    destruct H' as [[k' a'] [HxinPM H']].
-    apply fmap_Some_1 in H'.
-    destruct H' as [k'' [H1 H2]]. inversion H2. subst. clear H2.
-    assert (Hk': k' = encode k'').
-    { apply bool_decide_unpack in PMwf.
-      unfold map_Forall in PMwf.
-      apply pmap_to_list_lookup in HxinPM.
-      specialize (PMwf k' a' HxinPM).
-      apply (inj Some). rewrite <- PMwf.
-      apply fmap_Some_2. apply H1. }
-    subst. apply HxinPM.
-    
-  + apply pmap_to_list_lookup in H'.
-    apply elem_of_list_omap.
-    exists (encode k, a). firstorder.
-    rewrite -> decode_encode. simpl. reflexivity.
-Qed.
-
-Program Instance inj_unit_r : @Inj (K * ()) K (@eq (K * ())) (@eq K) (@fst K ()).
-Next Obligation.
-  intros. destruct x,y. simpl in H. subst. destruct u. destruct u0. reflexivity.
-Defined.
-
-Lemma gset_to_list_elem_of `{Countable K} (S : gset K) (k : K) : k ∈ (mapset_elements S) <-> k ∈ S.
-Proof.
-  unfold mapset_elements.
-  destruct S as [M].
-  unfold elem_of at 2.
-  unfold gset_elem_of. unfold mapset_elem_of. simpl.
-  rewrite <- gmap_to_list_lookup.
-  unfold map_to_list.
-  assert (Hk : k = fst (k, ())).
-  { reflexivity. }
-  rewrite -> Hk at 1.
-  split; intros H'.
-  + apply elem_of_list_fmap_2_inj in H'. apply H'.
-    apply inj_unit_r.
-  + apply elem_of_list_fmap_1. assumption.
-Qed.
-
-(* TODO be more general then just EVarSet *)
-Lemma mapset_elements_to_set (X : EVarSet) : list_to_set (mapset_elements X) = X.
-Proof.
-  apply (iffRL (@mapset_eq evar (gmap evar) _ _ _ _ _ _ _ _ gmap_finmap _ _)).
-  intros x. 
-  pose proof (H' := @elem_of_list_to_set evar EVarSet _ _ _ _ _ x (mapset_elements X)).
-  rewrite -> H'. apply gset_to_list_elem_of.
-Qed.
-
-Lemma set_evar_fresh_is_fresh ϕ : evar_fresh (elements (free_evars ϕ)) ∉ free_evars ϕ.
-Proof.
+  unfold fresh_evar.
   intros H.
   pose proof (Hf := evar_fresh_is_fresh (elements (free_evars ϕ))).
+  unfold elements in H. unfold gset_elements in H.
+  apply gset_to_list_elem_of in H.
+  unfold elements in Hf. unfold gset_elements in Hf.
+  apply elem_of_list_In in H. contradiction.
+Qed.
+
+Lemma set_svar_fresh_is_fresh ϕ : fresh_svar ϕ ∉ free_svars ϕ.
+Proof.
+  unfold fresh_svar.
+  intros H.
+  pose proof (Hf := svar_fresh_is_fresh (elements (free_svars ϕ))).
   unfold elements in H. unfold gset_elements in H.
   apply gset_to_list_elem_of in H.
   unfold elements in Hf. unfold gset_elements in Hf.
@@ -674,7 +689,7 @@ forall phi, wfc_body_ex phi -> well_formed_closed (patt_exists phi).
 Proof.
   intros. unfold wfc_body_ex in H. unfold well_formed_closed. simpl.
   unfold well_formed_closed in H.
-  apply (wfc_aux_body_ex_imp2 phi 0 0 (evar_fresh (elements (free_evars phi)))) in H. exact H.
+  apply (wfc_aux_body_ex_imp2 phi 0 0 (fresh_evar phi)) in H. exact H.
   clear H.
   apply set_evar_fresh_is_fresh.
 Qed.
@@ -692,7 +707,7 @@ Qed.
 
 (*Similarly to the section above but with mu*)
 Definition wfc_body_mu phi := forall X, 
-  ~List.In X (free_svars phi) -> well_formed_closed (svar_open 0 X phi).
+  X ∉ (free_svars phi) -> well_formed_closed (svar_open 0 X phi).
 
 (*Helper for wfc_mu_to_wfc_body*)
 Lemma wfc_aux_body_mu_imp1:
@@ -742,8 +757,8 @@ forall phi, wfc_body_mu phi -> well_formed_closed (patt_mu phi).
 Proof.
   intros. unfold wfc_body_mu in H. unfold well_formed_closed. simpl.
   unfold well_formed_closed in H.
-  apply (wfc_aux_body_mu_imp2 phi 0 0 (svar_fresh (free_svars phi))) in H. exact H.
-  apply svar_fresh_is_fresh.
+  apply (wfc_aux_body_mu_imp2 phi 0 0 (fresh_svar phi)) in H. exact H.
+  apply set_svar_fresh_is_fresh.
 Qed.
 
 (* From https://www.chargueraud.org/research/2009/ln/main.pdf in 3.4 (lc_abs_iff_body) *)
@@ -860,13 +875,13 @@ match p with
 | patt_imp ls rs => Ensembles.Union _ (Complement _ (pattern_interpretation evar_val svar_val ls))
                             (pattern_interpretation evar_val svar_val rs)
 | patt_exists p' =>
-  let x := evar_fresh (elements (free_evars p')) in
+  let x := fresh_evar p' in
   FA_Union
     (fun e => pattern_interpretation (update_evar_val x e evar_val)
                             svar_val
                             (evar_open 0 x p'))
 | patt_mu p' =>
-  let X := svar_fresh (free_svars p') in
+  let X := fresh_svar p' in
   @LeastFixpointOf (Ensemble (@Domain m)) OS L
     (fun S => pattern_interpretation evar_val
                             (update_svar_val X S svar_val)
@@ -938,7 +953,7 @@ Lemma pattern_interpretation_ex_simpl
       (evar_val : evar -> Domain m) (svar_val : svar -> Power (Domain m))
       (p : Pattern) :
   pattern_interpretation evar_val svar_val (patt_exists p) =
-  let x := evar_fresh (elements (free_evars p)) in
+  let x := fresh_evar p in
   FA_Union 
     (fun e => pattern_interpretation (update_evar_val x e evar_val)
                             svar_val
@@ -949,7 +964,7 @@ Lemma pattern_interpretation_mu_simpl
       (evar_val : evar -> Domain m) (svar_val : svar -> Power (Domain m))
       (p : Pattern) :
   pattern_interpretation evar_val svar_val (patt_mu p) =
-  let X := svar_fresh (free_svars p) in
+  let X := fresh_svar p in
   @LeastFixpointOf (Ensemble (@Domain m)) OS L
     (fun S => pattern_interpretation evar_val
                             (update_svar_val X S svar_val)
@@ -1019,11 +1034,11 @@ match C with
 end.
 
 Fixpoint free_evars_ctx (C : Application_context)
-  : (ListSet.set evar) :=
+  : (EVarSet) :=
 match C with
-| box => List.nil
-| ctx_app_l cc p prf => set_union evar_eq (free_evars_ctx cc) (elements (free_evars p))
-| ctx_app_r p cc prf => set_union evar_eq (elements (free_evars p)) (free_evars_ctx cc)
+| box => empty
+| ctx_app_l cc p prf => union (free_evars_ctx cc) (free_evars p)
+| ctx_app_r p cc prf => union (free_evars p) (free_evars_ctx cc)
 end.
 
 Definition patt_not (phi : Pattern) := patt_imp phi patt_bott.
@@ -1338,7 +1353,7 @@ Inductive ML_proof_system (theory : Theory) :
   | Ex_gen (phi1 phi2 : Pattern) (x : evar) :
       well_formed phi1 -> well_formed phi2 ->
       theory ⊢ (phi1 ---> phi2) ->
-      set_mem evar_eq x (elements (free_evars phi2)) = false ->
+      x ∉ (free_evars phi2) ->
       theory ⊢ (exists_quantify x phi1 ---> phi2)
 
 (* Frame reasoning *)
